James C - plowing into evaluation

isabelle/Chapter09.thy
@@ -12,6 +12,15 @@ datatype expr =
 | Lam type expr
 | Ap expr expr
 
+primrec free_vars :: "expr => nat set"
+where "free_vars (Var v) = {v}"
+    | "free_vars Zero = {}"
+    | "free_vars (Succ e) = free_vars e"
+    | "free_vars (Rec e0 e1 et) = free_vars e0 Un free_vars et Un 
+          ((%x. case x of 0 => 0 | Suc 0 => 0 | Suc (Suc k) => k) ` free_vars e1)"
+    | "free_vars (Lam t b) = (%x. case x of 0 => 0 | Suc k => k) ` free_vars b"
+    | "free_vars (Ap e1 e2) = free_vars e1 Un free_vars e2"
+
 primrec incr_from :: "nat => expr => expr"
 where "incr_from n (Var v) = Var (if v < n then v else Suc v)"
     | "incr_from n Zero = Zero"
@@ -46,6 +55,19 @@ inductive_cases [elim!]: "typecheck e (Rec x y z) t"
 inductive_cases [elim!]: "typecheck e (Lam x y) t"
 inductive_cases [elim!]: "typecheck e (Ap x y) t"
 
+lemma inv_var: "typecheck env (Var v) t ==> lookup env v = Some t" 
+by (induction env "Var v" t rule: typecheck.induct, simp)
+lemma inv_zer: "typecheck env Zero t ==> t = Nat" 
+by (induction env Zero t rule: typecheck.induct, simp)
+lemma inv_suc: "typecheck env (Succ n) t ==> t = Nat & typecheck env n Nat"
+by (induction env "Succ n" t rule: typecheck.induct, simp)
+lemma inv_rec: "typecheck env (Rec e0 e1 e) t ==> typecheck env e Nat & typecheck env e0 t & typecheck (extend_at (extend_at env 0 Nat) 0 t) e1 t"
+by (induction env "Rec e0 e1 e" t rule: typecheck.induct, simp)
+lemma inv_lam: "typecheck env (Lam r e) t ==> EX t'. t = Arr r t' & typecheck (extend_at env 0 r) e t'"
+by (induction env "Lam r e" t rule: typecheck.induct, simp)
+lemma inv_app: "typecheck env (Ap e1 e2) t ==> EX t2. typecheck env e1 (Arr t2 t) & typecheck env e2 t2"
+by (induction env "Ap e1 e2" t rule: typecheck.induct, auto)
+                        
 lemma [simp]: "typecheck env e t ==> typecheck (extend_at env n k) (incr_from n e) t"
 proof (induction env e t arbitrary: n rule: typecheck.induct)
 case tvar
@@ -55,7 +77,7 @@ next case tzer
 next case tsuc
   thus ?case by simp
 next case (trec env e e0 t e1)
-  hence "typecheck (extend_at (extend_at (extend_at env 0 type.Nat) 0 t) (Suc (Suc n)) k) (incr_from (Suc (Suc n)) e1) t" by simp
+  hence "typecheck (extend_at (extend_at (extend_at env 0 Nat) 0 t) (Suc (Suc n)) k) (incr_from (Suc (Suc n)) e1) t" by simp
   with trec show ?case by (simp add: extend_at_swap)
 next case (tlam env r b t)
   hence "typecheck (extend_at (extend_at env 0 r) (Suc n) k) (incr_from (Suc n) b) t" by simp
@@ -65,6 +87,36 @@ next case (tapp env e1 t2 t e2)
   moreover from tapp have "typecheck (extend_at env n k) (incr_from n e2) t2" by simp
   ultimately show ?case by simp
 qed
+
+lemma typecheck_nofree: "typecheck env e t ==> k ~: free_vars e ==> typecheck (extend env k v) e t"
+proof (induction env e t arbitrary: k rule: typecheck.induct)
+case tvar
+  thus ?case by simp
+next case tzer
+  thus ?case by simp
+next case tsuc
+  thus ?case by simp
+next case (trec env e e0 t e1)
+  have "Suc (Suc k) ~: free_vars e1"
+  proof auto
+    assume "Suc (Suc k) : free_vars e1"
+    hence "!!f. k = f (Suc (Suc k)) ==> k : f`free_vars e1" by simp
+    with trec show False by simp
+  qed
+  with trec show ?case by simp
+next case (tlam env r b t)
+  hence "Suc k ~: free_vars b"
+  proof auto
+    assume "Suc k : free_vars b"
+    hence "!!f. k = f (Suc k) ==> k : f`free_vars b" by simp
+    with tlam show False by simp
+  qed
+  with tlam show ?case by simp
+next case (tapp env e1 t2 t e2)
+  from tapp have "typecheck (extend env k v) e1 (Arr t2 t)" by simp
+  moreover from tapp have "typecheck (extend env k v) e2 t2" by simp
+  ultimately show ?case by simp
+qed 
 
 lemma typecheck_subst: "typecheck (extend env x t') e t ==> typecheck env e' t' ==> typecheck env (subst e e' x) t"
 proof (induction "extend env x t'" e t arbitrary: env e' x rule: typecheck.induct)
@@ -83,5 +135,78 @@ next case (tapp e1 t2 t e2)
   moreover from tapp have "typecheck env (subst e2 e' x) t2" by simp
   ultimately show ?case by simp
 qed 
+
+primrec is_val :: "expr => bool"
+where "is_val (Var v) = False"
+    | "is_val Zero = True"
+    | "is_val (Succ n) = is_val n"
+    | "is_val (Rec e0 e1 et) = False"
+    | "is_val (Lam t b) = True"
+    | "is_val (Ap e1 e2) = False"
+
+inductive eval :: "expr => expr => bool"
+where esuc [simp]: "eval n n' ==> eval (Succ n) (Succ n')"
+    | eap1 [simp]: "eval e1 e1' ==> eval (Ap e1 e2) (Ap e1' e2)"
+    | eap2 [simp]: "is_val e1 ==> eval e2 e2' ==> eval (Ap e1 e2) (Ap e1 e2')"
+    | eap3 [simp]: "is_val e2 ==> eval (Ap (Lam t b) e2) (subst b e2 0)"
+    | erc1 [simp]: "eval e e' ==> eval (Rec e0 e1 e) (Rec e0 e1 e')"
+    | erc2 [simp]: "eval (Rec e0 e1 Zero) e0"
+    | erc3 [simp]: "is_val e ==> eval (Rec e0 e1 (Succ e)) (subst (subst e1 e 1) (Rec e0 e1 e) 0)"
+
+lemma canonical_nat: "typecheck env e Nat ==> is_val e ==> e = Zero | (EX v. typecheck env v Nat & is_val v & e = Succ v)"
+by (induction e, auto)
+
+lemma canonical_arr: "typecheck env e (Arr t1 t2) ==> is_val e ==> (EX v. e = Lam t1 v & typecheck (extend_at env 0 t1) v t2)"
+by (induction e, auto)
+
+theorem preservation: "eval e e' ==> typecheck env e t ==> typecheck env e' t"
+proof (induction e e' arbitrary: t rule: eval.induct)
+case (esuc n n')
+  moreover from esuc have "t = Nat" by (simp add: inv_suc)
+  moreover from esuc have "typecheck env n Nat" by (simp add: inv_suc)
+  ultimately show ?case by simp
+next case (eap1 e1 e1' e2)
+  with eap1 have "EX t2. typecheck env e1' (Arr t2 t) & typecheck env e2 t2" by (auto simp add: inv_app)
+  thus ?case by auto
+next case eap2
+  thus ?case by auto
+next case (eap3 e2 r b)
+  hence "typecheck env (Ap (Lam r b) e2) t" by simp
+
+  have "typecheck env (subst b e2 0) t" sorry
+  thus ?case by simp
+next case erc1
+  thus ?case by auto
+next case (erc2 e0 e1)
+  from erc2 have "typecheck env Zero Nat & typecheck env e0 t & typecheck (extend_at (extend_at env 0 Nat) 0 t) e1 t" by (rule inv_rec)
+  thus ?case by simp
+next case (erc3 e e0 e1)
+  thus ?case sorry
+qed
+
+theorem progress: "typecheck env e t ==> env = empty_map ==> is_val e | (EX e'. eval e e')"
+proof (induct rule: typecheck.induct)
+case tvar
+  thus ?case by auto
+next case tzer
+  thus ?case by simp
+next case (tsuc env n)
+  thus ?case 
+  proof (cases "is_val n")
+  case True
+    thus ?thesis by simp
+  next case False
+    from tsuc False have "\<exists>a. eval n a" by simp
+    hence "\<exists>a. eval (Succ n) (Succ a)" sorry
+    thus ?thesis by auto
+  qed
+next case trec
+  thus ?case sorry
+next case tlam
+  thus ?case by simp
+next case tapp
+  thus ?case sorry
+qed 
+
 
 end
