isabelle/AssocList.thy
@@ -69,6 +69,12 @@ by (induction env, cases v, simp_all)
 lemma [simp]: "v >= n ==> lookup (extend_at env n k) (Suc v) = lookup env v" 
 by (induction env, cases v, simp_all)
 
+lemma [simp]: "extend_at empty_map n k = extend empty_map n k"
+apply (simp add: empty_map_def)
+apply (cases n)
+apply auto
+sorry
+
 lemma extend_at_swap: "extend_at (extend_at env 0 r) (Suc n) k = extend_at (extend_at env n k) 0 r"
 proof (induction env)
 case (ASSOC f)
@@ -116,7 +122,9 @@ qed
 lemma [simp]: "extend_at (extend env x k) 0 r = extend (extend_at env 0 r) (Suc x) k"
 proof (induction env)
 case (ASSOC f)
-  thus ?case sorry
+  have "(\<lambda>kp. case kp of 0 \<Rightarrow> if 0 = 0 then Some r else (f(x \<mapsto> k)) kp | Suc kpp \<Rightarrow> if Suc kpp < 0 then (f(x \<mapsto> k)) kp else if Suc kpp = 0 then Some r else (f(x \<mapsto> k)) kpp) =
+    ((\<lambda>kp. case kp of 0 \<Rightarrow> if 0 = 0 then Some r else f kp | Suc kpp \<Rightarrow> if Suc kpp < 0 then f kp else if Suc kpp = 0 then Some r else f kpp)(Suc x \<mapsto> k))" sorry
+  thus ?case by auto
 qed
 
 end
